

1. Consider the boundary value problem (12.1)-(12.2) with  $f(x) = 1/x$ . Using (12.3) prove that  $u(x) = -x \log(x)$ . This shows that  $u \in C^2(0,1)$  but  $u(0)$  is not defined and  $u', u''$  do not exist at  $x = 0$  ( $\Rightarrow$ : if  $f \in C^0(0,1)$ , but not  $f \in C^0([0,1])$ , then  $u$  does not belong to  $C^0([0,1])$ ).

$$-u''(x) = f(x), 0 < x < 1,$$

$$u(0) = u(1) = 0.$$

(pf) By (12.3), we have  $u(x) = x \int_0^1 (1-s) f(s) ds - \int_0^x (x-s) f(s) ds$

$$\begin{aligned} \text{for } f(x) = \frac{1}{x} \quad u(x) &= x \int_0^1 (1-s) \cdot \frac{1}{s} ds - \int_0^x (x-s) \cdot \frac{1}{s} ds \\ &= x \left( \ln s - s \Big|_0^1 \right) - \left( x \ln s - s \Big|_0^x \right) \\ &= x \left( -1 - \lim_{s \rightarrow 0} \ln s \right) - \left( x \ln x - x - \lim_{s \rightarrow 0} x \ln s \right) \\ &= -x - x \ln x + x = -x \ln x \end{aligned}$$

6. Prove that  $G^k(x_j) = hG(x_j, x_k)$ , where  $G$  is Green's function introduced in (12.4) and  $G^k$  is its corresponding discrete counterpart solution of (12.4).

[Solution: we prove the result by verifying that  $L_h G = h e^k$ . Indeed, for a fixed  $x_k$  the function  $G(x_k, s)$  is a straight line on the intervals  $[0, x_k]$  and  $[x_k, 1]$  so that  $L_h G = 0$  at every node  $x_l$  with  $l = 0, \dots, k-1$  and  $l = k+1, \dots, n+1$ . Finally, a direct computation shows that  $(L_h G)(x_k) = 1/h$  which concludes the proof.]

$$G(x, s) = \begin{cases} s(1-x) & \text{if } 0 \leq s \leq x, \\ x(1-s) & \text{if } x \leq s \leq 1. \end{cases} \quad (12.4)$$

We have defined  $L_h G^k = e^k$

For any fixed  $s = x_k$ ,  $x \mapsto G(x, s)$  is linear on  $[0, s]$  and  $[s, 1]$

$$\Rightarrow (L_h G)_j = 0 \text{ for } j \neq k$$

$$\begin{aligned} \text{For } j=k: (L_h G)_k &= \frac{-G(x_{k-1}, s) + 2G(x_k, s) - G(x_{k+1}, s)}{h^2} \\ &= \frac{-x_{k-1}(1-s) + 2s(1-s) - s(1-x_{k+1})}{h^2} \\ &= \frac{-(k-1)h(1-kh) + 2kh(1-kh) - kh(1-(k+1)h)}{h^2} \\ &= \frac{1}{h} \end{aligned}$$

$$\begin{aligned} \Rightarrow (L_h G)_l &= \begin{cases} \frac{1}{h} & \text{if } l=k \\ 0 & \text{if } l \neq k \end{cases} \Rightarrow (L_h G) = \frac{1}{h} e^k \\ &\Rightarrow L_h(hG) = e^k \end{aligned}$$

$$\Rightarrow hG = G^k \quad (hG(x_j, x_k) = G^k(x_j)) \quad \square$$